Verbatim/lexer/impl_pref.v
@@ -1,0 +1,75 @@
+Require Import List.
+Import ListNotations.
+Require Import PeanoNat.
+Require Import Coq.omega.Omega.
+Require Import Coq.Numbers.NatInt.NZOrder.
+
+From Verbatim Require Import ltac.
+From Verbatim Require Import state.
+
+Module ImplFn (Import ST : state.T).
+
+  Import ST.Ty.
+  Import ST.Defs.
+
+  (* Invariant: index == length s *)
+  Fixpoint max_pref_fn (s : String) (i : index) (state : State)
+    : option (Prefix * Suffix * index):=
+    match s with
+    (* in a regex approach, accepting := nullable *)
+    | [] => if accepting state then Some ([],[],i) else None
+    | a :: s' =>
+      let
+        (* in a regex approach, transition := derivative *)
+        state' := transition a state in
+      let
+        mpxs := max_pref_fn s' (decr i) state' in
+
+      match mpxs with
+      | None => if (accepting state') then Some ([a], s', (decr i)) else
+                 if (accepting state) then Some ([], s, i) else
+                   None
+      | Some (p, q, qi) => Some (a :: p, q, qi)
+      end
+    end.
+
+  Definition extract_fsm_for_max (code : String) (i : index)
+             (sru : (Label * State)) :=
+    match sru with
+      (a, fsm) => (a, max_pref_fn code i fsm)
+    end.
+
+  Definition max_prefs (code : String) (i : index)
+             (erules : list (Label * State))
+    :=
+      map (extract_fsm_for_max code i) erules.
+
+  (* prefixes closest to the head are preferred *)
+  Definition longer_pref (apref1 apref2 : Label * (option (Prefix * Suffix * index)))
+    : Label * (option (Prefix * Suffix * index)) :=
+    match apref1, apref2 with
+    | (_, None), (_, _) => apref2
+    | (_, _), (_, None) => apref1
+    (* This is finding the min right now... *)
+    | (_, Some (x, _, _)), (_, Some (y, _, _)) => if (length x) =? (length y)
+                                                 then apref1 else
+                                                   if (length x) <? (length y)
+                                                   then apref2 else apref1
+    end.
+
+
+  Fixpoint max_of_prefs (mprefs : list (Label * (option (Prefix * Suffix * index))))
+    : Label * option (Prefix * Suffix * index) :=
+    match mprefs with
+    | [] => ([], @None (String * String * index))
+    | p :: ps => longer_pref p (max_of_prefs ps)
+    end.
+
+  
+  Definition init_srule (rule : Rule) : sRule :=
+    match rule with
+    | (label, re) => (label, init_state re)
+    end.
+
+
+End ImplFn.
