Verbatim/memo/correctness.v
@@ -12,9 +12,11 @@ Module CorrectFn (Import MEM : memo.T).
 
   Import MEM.STT.Defs.
   Import MEM.Defs.
+  Import MEM.Defs.Invariants.
   Module Import IMPL := ImplFn MEM.
   Import MEM.Defs.NaiveLexerF.LEM.IMPL.Lex.
   Import MEM.Defs.NaiveLexerF.LEM.
+  Import MEM.Defs.NaiveLexerF.LEM.Lemmas.
   Import MEM.Defs.NaiveLexerF.
   Import MEM.Defs.NaiveLexer.MPref.
   Import IMPL.
@@ -23,51 +25,64 @@ Module CorrectFn (Import MEM : memo.T).
   Module Export CaseLemmas.
 
     Lemma lex'_eq_body__M :
-      forall rules code Ms
+      forall (orig : String)
+        (Ms : list Memo)
+        (rules : list (sRule))
+        (code : String)
+        (i : index)
+        (Hindex : ith_suffix orig code i)
         (Ha : Acc lt (length code))
-        (Hlexy : lexy_list (zip Ms (map ssnd rules)))
+        (Hlexy : lexy_list orig (zip Ms (map ssnd rules)))
         (Hlen : length Ms = length rules),
-        (lex'__M Ms rules code Ha Hlexy Hlen =
-         (match max_of_prefs__M (max_prefs__M Ms code rules) as mpref'
-                return max_of_prefs__M (max_prefs__M Ms code rules) = mpref' -> _
+        (lex'__M orig Ms rules code i Hindex Ha Hlexy Hlen =
+         (match max_of_prefs__M (max_prefs__M Ms code i rules) as mpref'
+                return max_of_prefs__M (max_prefs__M Ms code i rules) = mpref' -> _
           with
           | (Ms', _, None) => fun _ => (Ms', [], code) (* Code cannot be processed further *)
-          | (Ms', _, Some ([], _)) => fun _ => (Ms', [], code) (* Code cannot be processed further *)
-          | (Ms', label, Some (ph :: pt, suffix)) =>
+          | (Ms', _, Some ([], _, _)) => fun _ => (Ms', [], code) 
+          | (Ms', label, Some (ph :: pt, suffix, i')) =>
             fun Heq =>
-              match (lex'__M Ms' rules suffix
-                           (acc_recursive_call__M _ _ _ _ _ _ _ _ Ha Hlexy Hlen Heq)
-                           (lexy_recursive_call _ _ _ _ _ _ _ _ Hlexy Hlen Heq)
-                           (len_recursive_call _ _ _ _ _ _ _ _ Hlen Heq)
+              let Hindex' := (index_rec_call__M _ _ _ _ _ _ _ _ _ _ _ Hlexy Hlen Heq Hindex) in
+              match (lex'__M orig Ms' rules suffix i'
+                       Hindex'
+                       (acc_recursive_call__M _ _ _ _ _ _ _ _ _ _ _ Ha Hlexy Hlen Heq Hindex Hindex')
+                       (lexy_recursive_call _ _ _ _ _ _ _ _ _ _ _ Hlexy Hlen Heq Hindex Hindex')
+                       (len_recursive_call _ _ _ _ _ _ _ _ _ _ Hlen Heq)
                     )
               with
               | (Ms'', lexemes, rest) => (Ms'', ((label, ph :: pt) :: lexemes), rest)
               end
           end eq_refl)).
     Proof. 
-      intros rules code Ha Hlexy Hlen.
-      destruct Ha; destruct Hlexy; auto.
+      intros orig Ms rules code i Hindex Ha Hlexy Hlen.
+      destruct Ha. auto.
     Qed.
 
     Lemma lex'_cases_backward__M :
-      forall (Ms : list Memo)
-        (rules : list sRule)
+      forall (orig : String)
+        (Ms : list Memo)
+        (rules : list (sRule))
         (code : String)
+        (i : index)
+        (Hindex : ith_suffix orig code i)
         (Ha : Acc lt (length code))
-        (Hlexy : lexy_list (zip Ms (map ssnd rules)))
+        (Hlexy : lexy_list orig (zip Ms (map ssnd rules)))
         (Hlen : length Ms = length rules)
-        (pr : list Memo * Label * option (Prefix * Suffix))
+        (pr : list Memo * Label * option (Prefix * Suffix * index))
         (res : list Memo * list Token * String)
-        (Heq : max_of_prefs__M (max_prefs__M Ms code rules) = pr),
-        match pr as mpref' return max_of_prefs__M (max_prefs__M Ms code rules) = mpref' -> _ with
+        (Heq : max_of_prefs__M (max_prefs__M Ms code i rules) = pr),
+        match pr as mpref' return max_of_prefs__M (max_prefs__M Ms code i rules) = mpref' -> _ with
         | (Ms', _, None) => fun _ => (Ms', [], code) (* Code cannot be processed further *)
-        | (Ms', _, Some ([], _)) => fun _ => (Ms', [], code) (* Code cannot be processed further *)
-        | (Ms', label, Some (h :: t, suffix)) =>
+        | (Ms', _, Some ([], _, _)) => fun _ => (Ms', [], code)
+        | (Ms', label, Some (h :: t, suffix, i')) =>
           fun Heq =>
-            match (lex'__M Ms' rules suffix
-                         (acc_recursive_call__M _ _ _ _ _ _ _ _ Ha Hlexy Hlen Heq)
-                         (lexy_recursive_call _ _ _ _ _ _ _ _ Hlexy Hlen Heq)
-                         (len_recursive_call _ _ _ _ _ _ _ _ Hlen Heq)
+            let Hindex' := (index_rec_call__M _ _ _ _ _ _ _ _ _ _ _ Hlexy Hlen Heq Hindex) in
+            match (lex'__M orig Ms' rules suffix i'
+                         Hindex'
+                         (acc_recursive_call__M _ _ _ _ _ _ _ _ _ _ _
+                                              Ha Hlexy Hlen Heq Hindex Hindex')
+                         (lexy_recursive_call _ _ _ _ _ _ _ _ _ _ _ Hlexy Hlen Heq Hindex Hindex')
+                         (len_recursive_call _ _ _ _ _ _ _ _ _ _ Hlen Heq)
                   )
             with
             | (Ms'', lexemes, rest) => (Ms'', ((label, h :: t) :: lexemes), rest)
@@ -76,41 +91,58 @@ Module CorrectFn (Import MEM : memo.T).
         -> match res with
           | (_, [], code') =>
             code' = code
-            /\ (snd (max_of_prefs__M (max_prefs__M Ms code rules)) = None
-               \/ exists suf, snd (max_of_prefs__M (max_prefs__M Ms code rules)) = Some ([], suf))
+            /\ (snd (max_of_prefs__M (max_prefs__M Ms code i rules)) = None
+               \/ exists suf, snd (max_of_prefs__M (max_prefs__M Ms code i rules))
+                        = Some ([], suf, init_index (length suf)))
           | (_, (label, prefix) :: lexemes, rest) =>
-            exists Ms'' Ms' h t suffix (Heq' : max_of_prefs__M (max_prefs__M Ms code rules)
-                                 = (Ms', label, Some (h :: t, suffix))),
-            lex'__M Ms' rules suffix
-                         (acc_recursive_call__M _ _ _ _ _ _ _ _ Ha Hlexy Hlen Heq')
-                         (lexy_recursive_call _ _ _ _ _ _ _ _ Hlexy Hlen Heq')
-                         (len_recursive_call _ _ _ _ _ _ _ _ Hlen Heq')
+            exists Ms'' Ms' h t suffix i' Hindex'
+              (Heq' : max_of_prefs__M (max_prefs__M Ms code i rules)
+                      = (Ms', label, Some (h :: t, suffix, i'))),
+            lex'__M orig Ms' rules suffix i'
+                  Hindex'
+                  (acc_recursive_call__M _ _ _ _ _ _ _ _ _ _ _
+                                       Ha Hlexy Hlen Heq' Hindex Hindex')
+                  (lexy_recursive_call _ _ _ _ _ _ _ _ _ _ _ Hlexy Hlen Heq' Hindex Hindex')
+                  (len_recursive_call _ _ _ _ _ _ _ _ _ _ Hlen Heq')
             = (Ms'', lexemes, rest)
             /\ h :: t = prefix
           end.
     Proof.
       intros.
       repeat dm; intros; subst; simpl in *; try congruence.
-      - split; inv H; eauto. right. exists s. apply f_equal with (f := snd) in Heq. auto.
-      - inv H. exists l3. exists l. exists s0. exists p2. exists s. exists Heq. split; auto.
+      - split; inv H; eauto. right. exists s.
+        assert(i0 = init_index (length s)).
+        {
+          eapply index_rec_call__M_gen in Heq; eauto. inv Heq. auto.
+        } 
+        rewrite H in *.
+        apply f_equal with (f := snd) in Heq. auto.
+      - repeat dm. inv H.
+      - repeat dm. inv H. exists l1. exists l. exists s0. exists p3. exists s. exists i0.
+        exists (index_rec_call__M code rules Ms l4 s0 p3 s l i i0 orig Hlexy Hlen Heq Hindex).
+        exists Heq. split; auto.
       - split; inv H; eauto. left. apply f_equal with (f := snd) in Heq. auto.
     Qed.
 
     Lemma lex'_cases__M :
-      forall Ms rules code Ha Hlexy Hlen res,
-        lex'__M Ms rules code Ha Hlexy Hlen = res
+      forall Ms rules code orig  i Hindex Ha Hlexy Hlen res,
+        lex'__M orig Ms rules code i Hindex Ha Hlexy Hlen = res
         -> match res with
           | (_, [], code') =>
             code' = code
-            /\ (snd (max_of_prefs__M (max_prefs__M Ms code rules)) = None
-               \/ exists suf, snd (max_of_prefs__M (max_prefs__M Ms code rules)) = Some ([], suf))
+            /\ (snd (max_of_prefs__M (max_prefs__M Ms code i rules)) = None
+               \/ exists suf, snd (max_of_prefs__M (max_prefs__M Ms code i rules))
+                        = Some ([], suf, init_index (length suf)))
           | (_, (label, prefix) :: lexemes, rest) =>
-            exists Ms'' Ms' h t suffix (Heq' : max_of_prefs__M (max_prefs__M Ms code rules)
-                                 = (Ms', label, Some (h :: t, suffix))),
-            lex'__M Ms' rules suffix
-                         (acc_recursive_call__M _ _ _ _ _ _ _ _ Ha Hlexy Hlen Heq')
-                         (lexy_recursive_call _ _ _ _ _ _ _ _ Hlexy Hlen Heq')
-                         (len_recursive_call _ _ _ _ _ _ _ _ Hlen Heq')
+            exists Ms'' Ms' h t suffix i' Hindex'
+              (Heq' : max_of_prefs__M (max_prefs__M Ms code i rules)
+                      = (Ms', label, Some (h :: t, suffix, i'))),
+            lex'__M orig Ms' rules suffix i'
+                  Hindex'
+                  (acc_recursive_call__M _ _ _ _ _ _ _ _ _ _ _
+                                       Ha Hlexy Hlen Heq' Hindex Hindex')
+                  (lexy_recursive_call _ _ _ _ _ _ _ _ _ _ _ Hlexy Hlen Heq' Hindex Hindex')
+                  (len_recursive_call _ _ _ _ _ _ _ _ _ _ Hlen Heq')
             = (Ms'', lexemes, rest)
             /\ h :: t = prefix
           end.
@@ -122,93 +154,87 @@ Module CorrectFn (Import MEM : memo.T).
 
   End CaseLemmas.
 
-  Lemma momprefs_memo_F : forall code rus l o Ms Ms' l' o',
-      max_of_prefs (max_prefs code rus) = (l, o)
-      -> max_of_prefs__M (max_prefs__M Ms code rus) = (Ms', l', o')
-      -> lexy_list (zip Ms (map ssnd rus))
+  Lemma momprefs_memo_F : forall code rus l o Ms Ms' l' o' orig i,
+      max_of_prefs (max_prefs code i rus) = (l, o)
+      -> max_of_prefs__M (max_prefs__M Ms code i rus) = (Ms', l', o')
+      -> lexy_list orig (zip Ms (map ssnd rus))
       -> length Ms = length rus
+      -> ith_suffix orig code i
       -> (l, o) = (l', o').
   Proof.
-    intros. destruct (max_prefs__M Ms code rus) eqn:E.
-    apply mprefs_memo_F in E; auto.
-    assert(max_prefs code rus = l1).
-    {
-      rewrite E. auto.
-    }
-    rewrite <- H3 in H0.
-    sis.
-    assert (Defs.NaiveLexer.MPref.max_of_prefs (max_prefs code rus)
-            = max_of_prefs (max_prefs code rus)).
+    intros. destruct (max_prefs__M Ms code i rus) eqn:E.
+    eapply mprefs_memo_F in E; eauto.
+    assert(A : max_prefs code i rus = l1).
     {
       auto.
     }
-    rewrite H3 in *. clear H3.
-    destruct (max_of_prefs (max_prefs code rus)).
+    rewrite <- A in H0.
+    sis.
+    assert (A0 : Defs.NaiveLexer.MPref.max_of_prefs (max_prefs code i rus)
+            = max_of_prefs (max_prefs code i rus)).
+    {
+      auto.
+    }
+    rewrite A in *. clear A.
+    destruct (max_of_prefs (max_prefs code i rus)).
     destruct (Defs.NaiveLexer.MPref.max_of_prefs l1).
-    inv H0. auto.
+    inv H0. rewrite H in *. auto.
   Qed.
 
-  Lemma lex'_memo_eq_ts : forall ts ts' code
+  Lemma lex'_memo_eq_ts : forall ts ts' code orig i Hindex Hindex'
                            (Ha Ha' : Acc lt (length code))
                            rus rest rest' iMs Ms Hlexy Hlen,
-    lex' rus code Ha = (ts, rest)
-    -> lex'__M iMs rus code
+    lex' rus code i Hindex Ha = (ts, rest)
+    -> lex'__M orig iMs rus code i Hindex'
             Ha' Hlexy Hlen = (Ms, ts', rest')
     -> ts = ts'.
   Proof.
     induction ts; destruct ts'; auto;
     intros; apply lex'_cases in H; apply lex'_cases__M in H0.
-    - exfalso. destruct t. destruct H0 as (Ms'' & Ms' & h & y & suffix & Heq' & H0).
+    - exfalso. destruct t. destruct H0 as (Ms'' & Ms' & h & y & suffix & i' & Hindex0 & Heq' & H0).
       destruct H. destruct H1.
       + clear H0.
-        destruct (max_of_prefs (max_prefs code rus)) eqn:E. simpl in H1.
-        assert(MPref.max_of_prefs (MPref.max_prefs code rus)
-               = max_of_prefs (max_prefs code rus)).
-        { auto. }
-        rewrite H0 in H1. clear H0.
-        rewrite E in H1. simpl in H1. rewrite H1 in *. clear H1.
-        apply momprefs_memo_F with (l := l0) (o := None) in Heq'; auto.
+        destruct (max_of_prefs (max_prefs code i rus)) eqn:E. simpl in H1.
+        rewrite H1 in *.
+        eapply momprefs_memo_F with (l := l0) (o := None) in Heq'; eauto.
         discriminate.
       + clear H0.
-        destruct (max_of_prefs (max_prefs code rus)) eqn:E. simpl in H1.
-        destruct H1.
-        assert(MPref.max_of_prefs (MPref.max_prefs code rus)
-               = max_of_prefs (max_prefs code rus)).
-        { auto. }
-        rewrite H1 in H0. clear H1. rewrite E in H0.
-        simpl in H0. rewrite H0 in *. clear H0.
-        apply momprefs_memo_F with (l := l0) (o := Some ([], x)) in Heq'; auto.
-        discriminate.
-    - exfalso. destruct a. destruct H as (h & t & suffix & Heq' & H).
+        destruct (max_of_prefs (max_prefs code i rus)) eqn:E. simpl in H1.
+        destruct H1. destruct H0.
+        eapply momprefs_memo_F in Heq'; eauto.
+        rewrite H0 in *. discriminate.
+    - exfalso. destruct a. destruct H as (h & t & suffix & i' & Heq' & H).
       destruct H. destruct H0. destruct H2.
-      + destruct (max_of_prefs__M (max_prefs__M iMs code rus)) eqn:E.
+      + destruct (max_of_prefs__M (max_prefs__M iMs code i rus)) eqn:E.
         simpl in H2. rewrite H2 in *. clear H2.
         destruct p0.
-        apply momprefs_memo_F with (l := l) (o := Some (h :: t, suffix)) in E; auto.
+        eapply momprefs_memo_F in E; eauto.
         discriminate.
-      + destruct (max_of_prefs__M (max_prefs__M iMs code rus)) eqn:E.
+      + destruct (max_of_prefs__M (max_prefs__M iMs code i rus)) eqn:E.
         destruct H2.
         simpl in H2. rewrite H2 in *. clear H2.
         destruct p0.
-        apply momprefs_memo_F with (l := l) (o := Some (h :: t, suffix)) in E; auto.
+        eapply momprefs_memo_F in E; eauto.
         discriminate.
     - destruct a. destruct t.
-      destruct H as (h & t & suffix & Heq & Hlex' & Hp).
-      destruct H0 as (Ms'' & Ms' & h0 & t0 & suffix0 & Heq0 & Hlex'0 & Hp0).
+      destruct H as (h & t & suffix & i' & Heq & Hlex' & Hp).
+      destruct H0 as (Ms'' & Ms' & h0 & t0 & suffix0 & i0 & Hindex'0 & Heq0 & Hlex'0 & Hp0).
       subst.
       assert (suffix = suffix0 -> ts = ts').
       {
+        assert(i' = i0).
+        { clear Hlex'. eapply momprefs_memo_F in Heq; eauto. repeat inj_all. auto. }
         intros. subst. eapply IHts; eauto.
       } 
       clear Hlex'0.
-      apply momprefs_memo_F with (l := l) (o := Some (h :: t, suffix)) in Heq0; auto.
+      eapply momprefs_memo_F in Heq0; eauto.
       inv Heq0. intros. subst. destruct H; reflexivity.
   Qed.
 
-  Lemma lex'_memo_splits : forall ts' ts code (Ha Ha' : Acc lt (length code))
+  Lemma lex'_memo_splits : forall ts' ts code orig i Hindex Hindex__M (Ha Ha' : Acc lt (length code))
                            rus rest rest' iMs Ms Hlexy Hlen,
-    lex' (map init_srule rus) code Ha = (ts, rest)
-    -> lex'__M iMs (map init_srule rus) code
+    lex' (map init_srule rus) code i Hindex Ha = (ts, rest)
+    -> lex'__M orig iMs (map init_srule rus) code i Hindex__M
          Ha' Hlexy Hlen = (Ms, ts', rest')
     -> code = (concat (map snd ts')) ++ rest'.
   Proof.
@@ -224,11 +250,14 @@ Module CorrectFn (Import MEM : memo.T).
     } 
     {
       apply lex'_cases__M in H0. destruct a.
-      destruct H0 as (Ms'' & Ms' & h0 & t0 & suffix0 & Heq0 & Hlex'0 & Hp0).
+      destruct H0 as (Ms'' & Ms' & h0 & t0 & suffix0 & i' & Hindex' & Heq0 & Hlex'0 & Hp0).
       apply lex'_cases in H. destruct t.
-      destruct H as (h & t & suffix & Heq & Hlex' & Hp).
+      destruct H as (h & t & suffix & i0 & Heq & Hlex' & Hp).
       assert(suffix = suffix0 -> code = concat (map snd ((l, p) :: ts')) ++ rest').
       {
+        assert(i0 = i').
+        { clear Hlex'. eapply momprefs_memo_F in Heq; eauto. repeat inj_all. auto. }
+        subst i0.
         intros. subst. eapply IHts' in Hlex'0; eauto.
         simpl. rewrite <- app_assoc. rewrite <- Hlex'0.
         eapply momprefs_memo_F in Heq0; eauto. clear Hlex'0. inv Heq0.
@@ -242,10 +271,10 @@ Module CorrectFn (Import MEM : memo.T).
       
       
   
-  Lemma lex'_memo_eq_rest : forall code (Ha Ha' : Acc lt (length code))
+  Lemma lex'_memo_eq_rest : forall code orig i Hindex Hindex' (Ha Ha' : Acc lt (length code))
                            ts rus rest ts' rest' iMs Ms Hlexy Hlen,
-    lex' (map init_srule rus) code Ha = (ts, rest)
-    -> lex'__M iMs (map init_srule rus) code
+    lex' (map init_srule rus) code i Hindex Ha = (ts, rest)
+    -> lex'__M orig iMs (map init_srule rus) code i Hindex'
          Ha' Hlexy Hlen = (Ms, ts', rest')
     -> rest = rest'.
   Proof.
@@ -259,10 +288,10 @@ Module CorrectFn (Import MEM : memo.T).
     rewrite H in *. apply app_inv_head in H0. auto.
   Qed.
 
-  Theorem lex'_memo_eq : forall code (Ha : Acc lt (length code))
+  Theorem lex'_memo_eq : forall code orig i Hindex Hindex' (Ha : Acc lt (length code))
                            ts rus rest ts' rest' Ms Hlexy Hlen,
-    lex' (map init_srule rus) code Ha = (ts, rest)
-    -> lex'__M (init_Memos (map init_srule rus)) (map init_srule rus) code
+    lex' (map init_srule rus) code i Hindex Ha = (ts, rest)
+    -> lex'__M orig (init_Memos (map init_srule rus)) (map init_srule rus) code i Hindex'
          Ha Hlexy Hlen = (Ms, ts', rest')
     -> (ts, rest) = (ts', rest').
   Proof.
@@ -280,12 +309,9 @@ Module CorrectFn (Import MEM : memo.T).
   Proof.
     intros. destruct (lex rus code) eqn:E.
     unfold lex__M. unfold lex in E.
-    destruct (lex'__M (init_Memos (map CorrectFn.IMPL.Lex.init_srule rus))
-       (map CorrectFn.IMPL.Lex.init_srule rus) code (lt_wf (length code))
-       (init_Memos_lexy (map CorrectFn.IMPL.Lex.init_srule rus))
-       (init_Memos_parallel (map CorrectFn.IMPL.Lex.init_srule rus))) eqn:E1.
+    repeat dm.
     destruct p.
-    apply lex'_memo_eq with (ts := l) (rest := s) in E1; auto.
+    eapply lex'_memo_eq in E0; eauto.
   Qed.
 
   Theorem lex_sound__M : forall ts code rest rus,
